Garden/Plonky3/keccak/columns.v
@@ -28,82 +28,59 @@ Module KeccakCols.
     a_prime_prime_0_0_bits : Array.t Z 64;
     a_prime_prime_prime_0_0_limbs : Array.t Z U64_LIMBS;
   }.
-
-  Module Valid.
-    Record t (x : t) : Prop := {
-      step_flags : Array.Valid.t (fun _ => True) x.(step_flags);
-      preimage : Array.Valid.t (Array.Valid.t (Array.Valid.t (fun _ => True))) x.(preimage);
-      a : Array.Valid.t (Array.Valid.t (Array.Valid.t (fun _ => True))) x.(a);
-      c : Array.Valid.t (Array.Valid.t (fun _ => True)) x.(c);
-      c_prime : Array.Valid.t (Array.Valid.t (fun _ => True)) x.(c_prime);
-      a_prime : Array.Valid.t (Array.Valid.t (Array.Valid.t (fun _ => True))) x.(a_prime);
-      a_prime_prime : Array.Valid.t (Array.Valid.t (Array.Valid.t (fun _ => True))) x.(a_prime_prime);
-      a_prime_prime_0_0_bits : Array.Valid.t (fun _ => True) x.(a_prime_prime_0_0_bits);
-      a_prime_prime_prime_0_0_limbs : Array.Valid.t (fun _ => True) x.(a_prime_prime_prime_0_0_limbs);
-    }.
-  End Valid.
 End KeccakCols.
 
-Module KeccakColsExplicit.
-  Record t : Set := {
-    step_flags : ExplicitArray.t Z NUM_ROUNDS;
-    export : Z;
-    preimage : ExplicitArray.t (ExplicitArray.t (ExplicitArray.t Z U64_LIMBS) 5) 5;
-    a : ExplicitArray.t (ExplicitArray.t (ExplicitArray.t Z U64_LIMBS) 5) 5;
-    c : ExplicitArray.t (ExplicitArray.t Z 64) 5;
-    c_prime : ExplicitArray.t (ExplicitArray.t Z 64) 5;
-    a_prime : ExplicitArray.t (ExplicitArray.t (ExplicitArray.t Z 64) 5) 5;
-    a_prime_prime : ExplicitArray.t (ExplicitArray.t (ExplicitArray.t Z U64_LIMBS) 5) 5;
-    a_prime_prime_0_0_bits : ExplicitArray.t Z 64;
-    a_prime_prime_prime_0_0_limbs : ExplicitArray.t Z U64_LIMBS;
-  }.
-End KeccakColsExplicit.
+Module Impl_KeccakCols.
+  (*
+  pub fn b(&self, x: usize, y: usize, z: usize) -> T {
+      debug_assert!(x < 5);
+      debug_assert!(y < 5);
+      debug_assert!(z < 64);
 
-Module StepFlagsInput.
-  Record t : Set := {
-    step_flag0 : Z;
-    step_flag1 : Z;
-    step_flag2 : Z;
-    step_flag3 : Z;
-    step_flag4 : Z;
-    step_flag5 : Z;
-    step_flag6 : Z;
-    step_flag7 : Z;
-    step_flag8 : Z;
-    step_flag9 : Z;
-    step_flag10 : Z;
-    step_flag11 : Z;
-    step_flag12 : Z;
-    step_flag13 : Z;
-    step_flag14 : Z;
-    step_flag15 : Z;
-    step_flag16 : Z;
-    step_flag17 : Z;
-    step_flag18 : Z;
-    step_flag19 : Z;
-    step_flag20 : Z;
-    step_flag21 : Z;
-    step_flag22 : Z;
-    step_flag23 : Z;
-  }.
+      // B is just a rotation of A', so these are aliases for A' registers.
+      // From the spec,
+      //     B[y, (2x + 3y) % 5] = ROT(A'[x, y], r[x, y])
+      // So,
+      //     B[x, y] = f((x + 3y) % 5, x)
+      // where f(a, b) = ROT(A'[a, b], r[a, b])
+      let a = (x + 3 * y) % 5;
+      let b = x;
+      let rot = R[a][b] as usize;
+      self.a_prime[b][a][(z + 64 - rot) % 64]
+  }
+  *)
+  Definition b (self : KeccakCols.t) (x y z : Z) : Z :=
+    let a := (x + 3 * y) mod 5 in
+    let b := x in
+    let rot := (R.(Array.get) a).(Array.get) b in
+    ((self.(KeccakCols.a_prime).(Array.get) b).(Array.get) a).(Array.get) ((z + 64 - rot) mod 64).
 
-  Definition to_value (x : t) : Array.t Z NUM_ROUNDS :=
-    {|
-      Array.value :=
-        [ x.(step_flag0); x.(step_flag1); x.(step_flag2); x.(step_flag3); x.(step_flag4); x.(step_flag5);
-          x.(step_flag6); x.(step_flag7); x.(step_flag8); x.(step_flag9); x.(step_flag10); x.(step_flag11);
-          x.(step_flag12); x.(step_flag13); x.(step_flag14); x.(step_flag15); x.(step_flag16); x.(step_flag17);
-          x.(step_flag18); x.(step_flag19); x.(step_flag20); x.(step_flag21); x.(step_flag22); x.(step_flag23)
-        ]
-    |}.
-End StepFlagsInput.
+  (*
+  pub fn a_prime_prime_prime(&self, y: usize, x: usize, limb: usize) -> T {
+      debug_assert!(y < 5);
+      debug_assert!(x < 5);
+      debug_assert!(limb < U64_LIMBS);
 
-Module StepFlagsOutput.
+      if y == 0 && x == 0 {
+          self.a_prime_prime_prime_0_0_limbs[limb]
+      } else {
+          self.a_prime_prime[y][x][limb]
+      }
+  }
+  *)
+  Definition a_prime_prime_prime (self : KeccakCols.t) (y x limb : Z) : Z :=
+    if (y =? 0) && (x =? 0) then
+      (self.(KeccakCols.a_prime_prime_prime_0_0_limbs).(Array.get) limb)
+    else
+      ((self.(KeccakCols.a_prime_prime).(Array.get) y).(Array.get) x).(Array.get) limb.
+End Impl_KeccakCols.
+
+Module U64.
   Definition t : Set :=
     Z.
 
-  Definition to_value (x : t) : Array.t Z NUM_ROUNDS :=
-    Array.from_fn_pure (fun i =>
-      if i =? x then 1 else 0
-    ).
-End StepFlagsOutput.
+  Definition to_bits (x : t) : Array.t Z 64 :=
+    {|
+      Array.get i := Z.b2z (Z.testbit x i)
+    |}.
+End U64.
